src/proofs/no_slashable_attestations/supporting_lemmas/dv_next_preserves_ind_inv/invs_dv_next_4.dfy
@@ -63,7 +63,7 @@ module Invs_DV_Next_4
             s.dv_pubkey,
             s.all_nodes
         )    
-        && pred_rcvd_attestation_shares_is_in_all_messages_sent(s) 
+        && inv_rcvd_attestation_shares_is_in_all_messages_sent(s) 
         && inv_decided_value_of_consensus_instance_of_slot_k_is_for_slot_k(s)
         && inv_attestation_shares_to_broadcast_is_a_subset_of_all_messages_sent(s)      
         && inv_decided_value_of_consensus_instance_is_decided_by_quorum(s)    
